ROBINSON_PlusPlus/Meta.lean
@@ -27,3 +27,4 @@ import ROBINSON_PlusPlus.Meta.CodeDistinct
 import ROBINSON_PlusPlus.Meta.Induction
 import ROBINSON_PlusPlus.Meta.ProofChain
 import ROBINSON_PlusPlus.Meta.DerivCond
+import ROBINSON_PlusPlus.Meta.Representability2
